Finally finish TEMP_virt_to_phys_eq

theories/addr_reg.v
@@ -374,22 +374,34 @@ Qed.
 
 (* TEMPORARILY: virtual and physical addresses are a 1-to-1 mapping *)
 Program Definition TEMP_virt_to_phys (v: VirtAddr) : PhysAddr :=
-  match finz.of_z (finz.to_z (finz_of_virt_addr v)) with
-  | Some p => finz_to_phys_addr p
-  | None => _
-  end.
+  finz_to_phys_addr (finz.FinZ (finz.to_z (finz_of_virt_addr v)) _ _).
 Next Obligation. 
   intros.
-  unfold finz_of_virt_addr, finz.of_z in *.
-  destruct v as [f], f.
-  simpl in *.
-  rewrite -> Z.ltb_lt in finz_lt.
-  rewrite -> Z.leb_le in finz_nonneg.
-  apply Z.lt_le_trans with _ _ MemNumPhys in finz_lt; last exact phys_fits_in_virt.
-  destruct (Z.lt_dec z MemNumPhys); last contradiction.
-  destruct (Z.le_dec 0%Z z); last contradiction.
-  discriminate.
+  destruct v as [f].
+  unfold finz_of_virt_addr.
+  generalize (finz_spec f); intros [lt nz].
+  apply Z.lt_le_trans with _ _ MemNumPhys in lt; last exact phys_fits_in_virt.
+  rewrite -> Z.ltb_lt.
+  assumption.  
 Defined.
+Next Obligation.
+  intros.
+  destruct v as [f].
+  unfold finz_of_virt_addr.
+  generalize (finz_spec f); intros [lt nz].
+  rewrite -> Z.leb_le.
+  assumption.
+Defined.
+
+  (* generalize (finz_spec f); intros [lt nz].
+  apply Z.lt_le_trans with _ _ MemNumPhys in lt; last exact phys_fits_in_virt.
+  unfold finz_of_virt_addr, finz.of_z in *.
+  destruct (Z.lt_dec f MemNumPhys), (Z.le_dec 0%Z f).
+  - discriminate.
+  - contradiction.
+  - contradiction.
+  - contradiction.
+Defined. *)
 
 (* Proof.
   apply finz_to_phys_addr.
@@ -402,14 +414,73 @@ Defined.
   - exact phys_fits_in_virt.
 Qed. *)
 
-Lemma TEMP_virt_to_phys_eq (a b : VirtAddr) :
-  a = b ->
+Global Lemma TEMP_virt_to_phys_eq (a b : VirtAddr) :
+  a = b <->
   TEMP_virt_to_phys a = TEMP_virt_to_phys b.
 Proof.
-  intros. unfold TEMP_virt_to_phys in *. destruct a,b. rewrite H. auto.
+  split; intros.
+  - f_equal. done.
+  - inversion H. unfold finz_of_virt_addr in *. 
+  destruct a as [fa], b as [fb]. 
+  destruct fa as [za ltba nzba], fb as [zb ltbb nzbb].
+  simpl in *. subst zb.
+  repeat f_equal; apply eq_proofs_unicity; decide equality.
+Qed.
+  
+  
+  Unset Printing Notations.
+    apply (finz_unique fa fb _ _ _ _) in H1.
+    destruct fa as [za ltba nzba], fb as [zb ltbb nzbb]. simpl in *.
+  
+  
+  destruct (@finz_eq_dec MemNumVirt) with fa fb. auto. destruct n. 
+  
+  
+    destruct fa as [za ltba nzba], fb as [zb ltbb nzbb]. simpl in *.
+    subst zb.
+  Unset Printing Notations.
+  
+   f_equal. simpl in *. apply H1. 
+  
+  
+  
+  
+  destruct a as [fa], b as [fb].
+    generalize (finz_spec fa); intros [lta nza].
+    generalize (finz_spec fb); intros [ltb nzb].
+    destruct fa as [za ltba nzba], fb as [zb ltbb nzbb].
+    unfold TEMP_virt_to_phys, finz_of_virt_addr, finz_to_phys_addr, finz.of_z in *.
+    simpl in *.
+    Unset Printing Notations.
+    
+    destruct (Z.lt_dec).
+  
+  
+  
+    unfold TEMP_virt_to_phys, finz_of_virt_addr, finz_to_phys_addr, finz.of_z in H.
+    simpl in H.
+    destruct (Z.lt_dec) as [ | n].
+    +admit.
+    + unfold not in n.  
+    
+    destruct (Z.le_dec) as [ | n]; last destruct n.
+    destruct (Z.lt_dec) as [ | n]; last destruct n.
+    destruct (Z.le_dec) as [ | n]; last destruct n.
+  
+  
+    unfold TEMP_virt_to_phys, finz_of_virt_addr, finz_to_phys_addr, finz.of_z in H. simpl in H.
+    destruct (Z.lt_dec z MemNumPhys) as [ | n]; last destruct n.
+    destruct (Z.le_dec 0%Z z) as [ | n]; last destruct n.
+    destruct (Z.lt_dec z0 MemNumPhys) as [ | n]; last destruct n.
+    destruct (Z.le_dec 0%Z z0) as [ | n]; last destruct n.
+    (* destruct (Z.ltb_lt z MemNumPhys), (Z.ltb_lt z0 MemNumPhys), (Z.leb_le 0 z), (Z.leb_le 0 z0). *)
+    inversion H. subst z0.
+    generalize dependent finz_nonneg.
+    generalize dependent finz_nonneg0.
+    destruct ((z <? MemNumVirt)%Z).
 Qed.
 
-Lemma TEMP_virt_to_phys_neq (a b : VirtAddr) :
+Global Lemma TEMP_virt_to_phys_neq (a b : VirtAddr) :
   TEMP_virt_to_phys a ≠ TEMP_virt_to_phys b ->
   a ≠ b.
 Proof.
